examples/rv_cache_isolation/tests/enclave/mmio3.h
@@ -1,0 +1,10 @@
+#ifndef MMIO0_H
+#define MMIO0_H
+
+int getchar3();
+int putchar3(int c);
+void putchars3(const char* str);
+
+int getled3();
+int putled3(int on);
+#endif
