examples/rv_isolation/tests/enclave/enclave0.c
@@ -1,0 +1,83 @@
+#include "mmio0.h"
+
+static const char* pattern = "-.- --- .. -.- .-";
+
+#define DOT 20
+#define DASH (3 * DOT)
+#define SPACE DOT
+#define LETTER_SPACE (3 * DOT)
+#define WORD_SPACE (7 * DOT)
+
+static void wait(int duration) {
+  for (int i = 0; i < duration; i++);
+}
+
+static void blink(char c) {
+  int on, duration;
+
+  switch (c) {
+  case '.':
+    on = 1, duration = DOT;
+    break;
+  case '-':
+    on = 1, duration = DASH;
+    break;
+  default:
+    on = 0, duration = LETTER_SPACE;
+    break;
+  }
+
+  putled0(on);
+  wait(duration);
+  putled0(0);
+  wait(SPACE);
+}
+
+#define REPEAT 1
+
+/*
+int main0() {
+  for (int i = 0; i < REPEAT; i++) {
+    wait(WORD_SPACE);
+    const char* p = pattern;
+    while (*p)
+      blink(*p++);
+  }
+  putchar0('\n');
+}
+*/
+extern int _add_password(unsigned int id, char value, int secret);
+extern char _lookup(unsigned int id, int secret);
+
+
+int main0 () {
+  int secret_code = 42;
+
+  putchar0('1');
+  putchar0('-');
+  putchar0('>');
+  putchar0('S');
+  putchar0('@');
+  putchar0(secret_code);
+//  putchar0('\n');
+//  blink('.');
+//  blink('-');
+  // Switch to another enclave and add password
+  _add_password(1, 'S', secret_code);
+  // Switch to other enclave and lookup password
+  char ch = _lookup(1, secret_code);
+  // Output the result
+  putchar0(ch);
+//  blink('.');
+  // Lookup with the wrong secret
+  ch = _lookup(1, 0);
+  // Expect 0
+  putchar0(ch);
+
+  _add_password(1, 'T', secret_code);
+  ch = _lookup(1, secret_code);
+  putchar0(ch);
+
+//  blink('.');
+  putchar0('\n');
+}
