examples/rv_isolation/tests/enclave/mmio2.c
@@ -1,0 +1,33 @@
+static int* const UART_ADDR = (int*)0x40000000;
+static int* const LED_ADDR  = (int*)0x40000004;
+static int* const STOP_ADDR = (int*)0x40001000;
+
+int getchar2() {
+  return 0;
+}
+
+void __attribute__((noreturn)) exit2(int code) {
+  *STOP_ADDR = code;
+  __builtin_unreachable();
+}
+
+int putchar2(int c) {
+  *UART_ADDR = c;
+  return c;
+}
+
+int getled2() {
+  return *LED_ADDR;
+}
+
+int putled2(int on) {
+  *LED_ADDR = on;
+  return on;
+}
+
+static inline __attribute__((unused)) void putchars2(const char* str) {
+  while (*str) {
+    putchar2(*str);
+    str++;
+  }
+}
