examples/rv_cache_isolation/External.v
@@ -1,0 +1,88 @@
+Require Import Koika.Frontend.
+Require Import rv_cache_isolation.RVCore.
+Require Import rv_cache_isolation.Common.
+Require Import rv_cache_isolation.Machine.
+
+
+Module EnclaveParams <: EnclaveParams_sig.
+  Definition enclave_base (eid: enclave_id) : addr_t :=
+    Eval vm_compute in (
+    match eid with
+    | Enclave0 => Ob~0~0~0~0~0~0~0~0~0~0~0~0~0~0~0~0~0~0~0~0~0~0~0~0~0~0~0~0~0~0~0~0
+    | Enclave1 => Ob~0~0~0~0~0~0~0~0~0~0~0~0~0~0~0~0~0~1~0~0~0~0~0~0~0~0~0~0~0~0~0~0
+    | Enclave2 => Ob~0~0~0~0~0~0~0~0~0~0~0~0~0~0~0~0~1~0~0~0~0~0~0~0~0~0~0~0~0~0~0~0
+    | Enclave3 => Ob~0~0~0~0~0~0~0~0~0~0~0~0~0~0~0~0~1~1~0~0~0~0~0~0~0~0~0~0~0~0~0~0
+    end).
+ Definition enclave_size (eid: enclave_id) : bits_t 32 :=
+    Eval vm_compute in (
+                 Ob~0~0~0~0~0~0~0~0~0~0~0~0~0~0~0~0~0~1~0~0~0~0~0~0~0~0~0~0~0~0~0~0).
+ Definition enclave_bootloader_addr (eid: enclave_id) : addr_t :=
+    Eval vm_compute in (
+    match eid with
+    | Enclave0 => Ob~0~0~0~0~0~0~0~0~0~0~0~0~0~0~0~0~0~0~0~0~0~0~0~1~0~0~0~0~0~0~0~0
+    | Enclave1 => Ob~0~0~0~0~0~0~0~0~0~0~0~0~0~0~0~0~0~1~0~0~0~0~0~1~0~0~0~0~0~0~0~0
+    | Enclave2 => Ob~0~0~0~0~0~0~0~0~0~0~0~0~0~0~0~0~1~0~0~0~0~0~0~0~0~0~0~0~0~0~0~0
+    | Enclave3 => Ob~0~0~0~0~0~0~0~0~0~0~0~0~0~0~0~0~1~1~0~0~0~0~0~0~0~0~0~0~0~0~0~0
+    end).
+
+  Definition shared_region_base (id: shared_id) : addr_t :=
+    Eval vm_compute in (
+    match id with
+    | Shared01 =>
+        Ob~0~0~0~0~0~0~0~1~0~0~0~0~0~0~0~0~0~0~0~0~0~0~0~0~0~0~0~0~0~0~0~0
+    | Shared02 =>
+        Ob~0~0~0~0~0~0~0~1~0~0~0~0~0~0~0~0~1~0~0~0~0~0~0~0~0~0~0~0~0~0~0~0
+    | Shared03 =>
+        Ob~0~0~0~0~0~0~0~1~0~0~0~0~0~0~0~1~0~0~0~0~0~0~0~0~0~0~0~0~0~0~0~0
+    | Shared12 =>
+        Ob~0~0~0~0~0~0~0~1~0~0~0~0~0~0~0~1~1~0~0~0~0~0~0~0~0~0~0~0~0~0~0~0
+    | Shared13 =>
+        Ob~0~0~0~0~0~0~0~1~0~0~0~0~0~0~1~0~0~0~0~0~0~0~0~0~0~0~0~0~0~0~0~0
+    | Shared23 =>
+        Ob~0~0~0~0~0~0~0~1~0~0~0~0~0~0~1~0~1~0~0~0~0~0~0~0~0~0~0~0~0~0~0~0
+    end).
+
+  Definition shared_region_size : bits_t 32 :=
+    Eval vm_compute in (
+        Ob~0~0~0~0~0~0~0~0~0~0~0~0~0~0~0~0~1~0~0~0~0~0~0~0~0~0~0~0~0~0~0~0).
+
+  Definition core_init0 : core_init_params_t :=
+    Eval vm_compute in (
+    {| machine_pc := Ob~0~0~0~0~0~0~0~0~0~0~0~0~0~0~0~0~0~0~0~0~0~0~0~0~0~0~0~0~0~0~0~0;
+       machine_config := Some {| config_eid := Enclave0;
+                                 config_shared_regions := fun sid =>
+                                                            match sid with
+                                                            | Shared01 => true
+                                                            | Shared02 => true
+                                                            | Shared03 => true
+                                                            | _ => false
+                                                            end;
+                                 config_ext_uart := true;
+                                 config_ext_led := true;
+                                 config_ext_finish := true
+                              |}
+    |}).
+
+  Definition core_init1 : core_init_params_t :=
+    Eval vm_compute in (
+    {| machine_pc := Ob~0~0~0~0~0~0~0~0~0~0~0~0~0~0~0~0~0~1~0~0~0~0~0~0~0~0~0~0~0~0~0~0;
+       machine_config := Some {| config_eid := Enclave1;
+                                 config_shared_regions := fun _ => false;
+                                 config_ext_uart := false;
+                                 config_ext_led := false;
+                                 config_ext_finish := false
+                              |}
+    |}).
+
+  Definition enclave_params: enclave_params_sig :=
+  {| _enclave_base := enclave_base;
+     _enclave_size := enclave_size;
+     _enclave_bootloader_addr := enclave_bootloader_addr;
+     _shared_region_base :=shared_region_base;
+     _shared_region_size := shared_region_size;
+     _core_init0 := core_init0;
+     _core_init1 :=  core_init1;
+  |}.
+
+
+End EnclaveParams.
