examples/rv_isolation/MemoryWithCache.v
@@ -1,0 +1,457 @@
+(*! Deprecated *)
+(*
+Require Import Koika.Frontend.
+Require Import Koika.Std.
+Require Import Coq.Lists.List.
+Require Import rv_isolation.Common.
+
+Inductive mem_rules_t :=
+| Rl_doMemReq (core: ind_core_id)
+| Rl_doMemResp (core: ind_core_id)
+| Rl_doPurge (core: ind_core_id)
+| Rl_doExternalMem
+| Rl_tick
+| Rl_doInit (core: ind_core_id).
+
+Module Type Memory_sig.
+  Parameter _reg_t : Type.
+  Parameter _ext_fn_t : Type.
+  Parameter R : _reg_t -> type.
+  Parameter Sigma : _ext_fn_t -> ExternalSignature.
+  Parameter r : bits_t 2 -> forall reg, R reg.
+  Parameter rules : mem_rules_t -> rule R Sigma.
+  Parameter FiniteType_reg_t : FiniteType _reg_t.
+  Parameter Show_reg_t : Show _reg_t.
+  Parameter schedule : @Syntax.scheduler Frontend.pos_t mem_rules_t.
+End Memory_sig.
+
+Definition NLINES := 512. (* 512 *)
+Definition data_sig := bits_t 32.
+Definition log_nlines := log2 NLINES.
+
+Definition shreq :=
+  {| struct_name := "shreq";
+     struct_fields := [("req" , struct_t mem_req);
+                       ("sourceType"    , bits_t 1);
+                       ("sourceCore"    , bits_t 1);
+                       ("valid"    , bits_t 1)
+                       ] |}.
+Definition shresp :=
+  {| struct_name := "shresp";
+     struct_fields := [("resp" , struct_t mem_resp);
+                       ("sourceType"    , bits_t 1);
+                       ("sourceCore"    , bits_t 1);
+                       ("valid"    , bits_t 1)
+                       ] |}.
+Definition mem_input :=
+  {| struct_name := "mem_input";
+     struct_fields := [("get_ready", bits_t 1);
+                      ("put_valid", bits_t 1);
+                      ("put_request", struct_t mem_req)] |}.
+
+Definition mem_output :=
+  {| struct_name := "mem_output";
+     struct_fields := [("get_valid", bits_t 1);
+                      ("put_ready", bits_t 1);
+                      ("get_response", struct_t mem_resp)] |}.
+
+  Definition cache_req_sig :=
+    {| struct_name := "cache_req";
+      struct_fields := [("byte_en", bits_t 4); ("addr", bits_t log_nlines); ("data", bits_t 32)] |}.
+  Definition cache_input_sig :=
+    {| struct_name := "cache_input";
+       struct_fields := [("get_ready", bits_t 1); ("put_valid", bits_t 1); ("put_request", struct_t cache_req_sig)]
+    |}.
+  Definition metadata_sig :=
+    {| struct_name := "cache_metadata";
+       struct_fields := [("tag", bits_t (log2 NLINES))
+                         ;("valid", bits_t 1 )]
+    |}.
+
+  Definition metadata_req_sig :=
+    {| struct_name := "metadata_req";
+       struct_fields := [("is_write", bits_t 1); ("addr", bits_t log_nlines); ("data", struct_t metadata_sig)] |}.
+
+  Definition metadata_input_sig :=
+    {| struct_name := "metadata_input";
+       struct_fields := [("get_ready", bits_t 1); ("put_valid", bits_t 1); ("put_request", struct_t metadata_req_sig)]
+    |}.
+
+  Definition cache_output_sig :=
+    {| struct_name := "cache_output";
+       struct_fields := [("get_valid", bits_t 1); ("put_ready", bits_t 1); ("get_response", data_sig)]
+    |}.
+  Definition metadata_output_sig :=
+    {| struct_name := "metadata_output";
+       struct_fields := [("get_valid", bits_t 1); ("put_ready", bits_t 1); ("get_response", struct_t metadata_sig)]
+    |}.
+
+Module Memory <: Memory_sig.
+  Inductive mem_type := imem | dmem.
+
+  Inductive ext_fn_t :=
+  | ext_cache_imem0
+  | ext_cache_imem1
+  | ext_cache_dmem0
+  | ext_cache_dmem1
+  | ext_metacache_imem0
+  | ext_metacache_imem1
+  | ext_metacache_dmem0
+  | ext_metacache_dmem1
+  | ext_mainmem
+  .
+
+  Definition Sigma (fn: ext_fn_t) :=
+  match fn with
+  | ext_cache_imem0 => {$ struct_t cache_input_sig ~> struct_t cache_output_sig $}
+  | ext_cache_imem1 => {$ struct_t cache_input_sig ~> struct_t cache_output_sig $}
+  | ext_cache_dmem0 => {$ struct_t cache_input_sig ~> struct_t cache_output_sig $}
+  | ext_cache_dmem1 => {$ struct_t cache_input_sig ~> struct_t cache_output_sig $}
+  | ext_metacache_imem0 => {$ struct_t metadata_input_sig ~> struct_t metadata_output_sig $}
+  | ext_metacache_imem1 => {$ struct_t metadata_input_sig ~> struct_t metadata_output_sig $}
+  | ext_metacache_dmem0 => {$ struct_t metadata_input_sig ~> struct_t metadata_output_sig $}
+  | ext_metacache_dmem1 => {$ struct_t metadata_input_sig ~> struct_t metadata_output_sig $}
+  | ext_mainmem => {$ struct_t mem_input ~> struct_t mem_output $}
+  end.
+
+  Inductive reg_t :=
+  | toIMem0 (state: MemReq.reg_t) (* These go to the caches *)
+  | toIMem1 (state: MemReq.reg_t)
+  | toDMem0 (state: MemReq.reg_t)
+  | toDMem1 (state: MemReq.reg_t)
+  | fromIMem0 (state: MemRespBypass.reg_t)
+  | fromIMem1 (state: MemRespBypass.reg_t)
+  | fromDMem0 (state: MemRespBypass.reg_t)
+  | fromDMem1 (state: MemRespBypass.reg_t)
+  | toMainMemIMem0 (state: MemReq.reg_t)
+  | toMainMemIMem1 (state: MemReq.reg_t)
+  | toMainMemDMem0 (state: MemReq.reg_t)
+  | toMainMemDMem1 (state: MemReq.reg_t)
+  | fromMainMemIMem0 (state: MemRespBypass.reg_t)
+  | fromMainMemIMem1 (state: MemRespBypass.reg_t)
+  | fromMainMemDMem0 (state: MemRespBypass.reg_t)
+  | fromMainMemDMem1 (state: MemRespBypass.reg_t)
+  | SHReq
+  | SHResp
+  | purge (core: ind_core_id)
+  | turn
+  | priv_turn (core: ind_core_id)
+  .
+
+  Definition R (idx: reg_t) : type :=
+    match idx with
+    | toIMem0 st => MemReq.R st
+    | toIMem1 st => MemReq.R st
+    | toDMem0 st => MemReq.R st
+    | toDMem1 st => MemReq.R st
+    | fromIMem0 st => MemRespBypass.R st
+    | fromIMem1 st => MemRespBypass.R st
+    | fromDMem0 st => MemRespBypass.R st
+    | fromDMem1 st => MemRespBypass.R st
+    | toMainMemIMem0 st => MemReq.R st
+    | toMainMemIMem1 st => MemReq.R st
+    | toMainMemDMem0 st => MemReq.R st
+    | toMainMemDMem1 st => MemReq.R st
+    | fromMainMemIMem0 st => MemRespBypass.R st
+    | fromMainMemIMem1 st => MemRespBypass.R st
+    | fromMainMemDMem0 st => MemRespBypass.R st
+    | fromMainMemDMem1 st => MemRespBypass.R st
+    | SHReq => struct_t shreq
+    | SHResp => struct_t shresp
+    | purge _ => enum_t purge_state
+    | turn => bits_t 2
+    (* | reg_metadata_req => maybe (struct_t metadata_input_sig) *)
+    (* | reg_metadata_resp => maybe (struct_t metadata_output_sig) *)
+    | priv_turn _=> bits_t 1
+    end.
+
+  Definition r (turn: bits_t 2) (idx: reg_t) : R idx :=
+    match idx with
+    | toIMem0 st => MemReq.r st
+    | toIMem1 st => MemReq.r st
+    | toDMem0 st => MemReq.r st
+    | toDMem1 st => MemReq.r st
+    | fromIMem0 st => MemRespBypass.r st
+    | fromIMem1 st => MemRespBypass.r st
+    | fromDMem0 st => MemRespBypass.r st
+    | fromDMem1 st => MemRespBypass.r st
+    | toMainMemIMem0 st => MemReq.r st
+    | toMainMemIMem1 st => MemReq.r st
+    | toMainMemDMem0 st => MemReq.r st
+    | toMainMemDMem1 st => MemReq.r st
+    | fromMainMemIMem0 st => MemRespBypass.r st
+    | fromMainMemIMem1 st => MemRespBypass.r st
+    | fromMainMemDMem0 st => MemRespBypass.r st
+    | fromMainMemDMem1 st => MemRespBypass.r st
+    | purge _ => value_of_bits (Bits.zero)
+    | turn => turn
+    | SHReq  => value_of_bits (Bits.zero)
+    | SHResp => value_of_bits (Bits.zero)
+    | priv_turn _ => Bits.zero
+    end.
+
+  Definition _reg_t := reg_t.
+  Instance FiniteType_reg_t : FiniteType _reg_t := _.
+  Definition _ext_fn_t := ext_fn_t.
+  (* Definition Sigma := Sigma. *)
+
+
+  Definition coreToCache (cache: mem_type) (core: ind_core_id) :=
+    fun reg => (match cache, core with
+            | imem, CoreId0 => toIMem0
+            | imem, CoreId1 => toIMem1
+            | dmem, CoreId0 => toDMem0
+            | dmem, CoreId1 => toDMem1
+            end) reg.
+
+  Definition toMainMem (cache: mem_type) (core: ind_core_id) :=
+    fun reg => (match cache, core with
+            | imem, CoreId0 => toMainMemIMem0
+            | imem, CoreId1 => toMainMemIMem1
+            | dmem, CoreId0 => toMainMemDMem0
+            | dmem, CoreId1 => toMainMemDMem1
+            end) reg.
+
+  Definition fromMainMem (cache: mem_type) (core: ind_core_id) :=
+    fun reg => (match cache, core with
+            | imem, CoreId0 => fromMainMemIMem0
+            | imem, CoreId1 => fromMainMemIMem1
+            | dmem, CoreId0 => fromMainMemDMem0
+            | dmem, CoreId1 => fromMainMemDMem1
+            end) reg.
+
+  Definition cacheToCore (cache: mem_type) (core: ind_core_id) :=
+    fun reg => (match cache, core with
+            | imem, CoreId0 => fromIMem0
+            | imem, CoreId1 => fromIMem1
+            | dmem, CoreId0 => fromDMem0
+            | dmem, CoreId1 => fromDMem1
+            end) reg.
+
+  Definition doCache (cache: mem_type) (core: ind_core_id) : uaction reg_t ext_fn_t :=
+    {{ guard(read0(purge core) == enum purge_state { Ready });
+       pass
+    }}.
+
+
+  Definition do_mem_req (core_id: ind_core_id): uaction reg_t ext_fn_t :=
+    let fromIMem := fromIMem core_id in
+    let toIMem := toIMem core_id in
+    let fromDMem := fromDMem core_id in
+    let toDMem := toDMem core_id in
+    {{ guard(read0(purge core_id) == enum purge_state { Ready } );
+       guard(read0(turn) == #(mem_write_turn core_id));
+       (if (read0(priv_turn core_id)) then
+         if ( fromIMem.(MemRespBypass.can_enq)() && toIMem.(MemReq.can_deq)())  then
+           (let req := toIMem.(MemReq.deq)() in
+            write0(SHReq, struct shreq { req := req;
+                                         sourceType := Ob~1;
+                                         sourceCore := (#(core_id_to_bits core_id));
+                                         valid := Ob~1
+                                        })
+           )
+         else
+           pass
+       else (* (read0(priv_turn core_id) == Ob~1 *)
+         if ( fromDMem.(MemRespBypass.can_enq)() && toDMem.(MemReq.can_deq)())  then
+           (let req := toDMem.(MemReq.deq)() in
+            write0(SHReq, struct shreq { req := req;
+                                         sourceType := Ob~0;
+                                         sourceCore := (#(core_id_to_bits core_id));
+                                         valid := Ob~1
+                                        })
+           )
+         else pass);
+       write0((priv_turn core_id), read0(priv_turn core_id) + Ob~1)
+    }}.
+
+  Definition do_mem_resp (core_id: ind_core_id) : uaction reg_t ext_fn_t :=
+    let fromIMem := fromIMem core_id in
+    let toIMem := toIMem core_id in
+    let fromDMem := fromDMem core_id in
+    let toDMem := toDMem core_id in
+    {{ guard(read0(purge core_id) == enum purge_state { Ready } );
+       guard(get(read1(SHResp), sourceCore) == #(core_id_to_bits core_id));
+       guard(get(read1(SHResp), valid) == Ob~1);
+       let resp := read1(SHResp) in
+       let iorD := get(resp, sourceType) in (* I is 1, D is 0 *)
+       let res := get(resp, resp) in
+       (if ((iorD == Ob~0) && fromDMem.(MemRespBypass.can_enq)()) then
+          fromDMem.(MemRespBypass.enq)(res)
+        else if ((iorD == Ob~1) && fromIMem.(MemRespBypass.can_enq)()) then
+          fromIMem.(MemRespBypass.enq)(res)
+        else pass)
+    }}.
+
+  Definition do_external_mem : uaction reg_t ext_fn_t :=
+    {{
+        let req := read1(SHReq) in
+        let enqueue := get(req, valid) in
+        let memory_request := (if enqueue then get(req, req)
+                               else `UConst (tau := struct_t mem_req) (value_of_bits Bits.zero)`) in
+        let response := extcall ext_mainmem (struct mem_input {get_ready := Ob~1;
+                                                               put_valid := enqueue;
+                                                               put_request := memory_request }) in
+        (if enqueue then
+           write1(SHReq, subst (req,valid,Ob~0))
+         else pass);
+        let is_response := get(response, get_valid) in
+        let response := get(response, get_response) in
+        write0(SHResp, struct shresp { resp := response;
+                                       sourceType := get(req, sourceType);
+                                       sourceCore := get(req, sourceCore);
+                                       valid := is_response })
+    }}.
+
+  Definition do_tick_turn : uaction reg_t ext_fn_t :=
+    {{ let turn := read0(turn) in
+      (* Tick in memory, every two cycles we can enqueue a new thing *)
+      (* write0(public turn, turn  + Ob~0~1); *)
+       write0(turn, turn + Ob~0~1)
+    }}.
+
+  Definition do_init (core_id: ind_core_id) : uaction reg_t ext_fn_t :=
+    {{ guard (read0(purge core_id) == enum purge_state { Init } );
+       write0(purge core_id, enum purge_state { Ready } )
+    }}.
+
+  Definition do_purge (core_id: ind_core_id) : uaction reg_t ext_fn_t :=
+    let toIMem := toIMem core_id in
+    let toDMem := toDMem core_id in
+    {{ guard(read0(purge core_id) == enum purge_state { Purging } );
+       guard(read0(turn) == #(cid_to_freeze_cycle core_id));
+       (* Reset private state *)
+       write0(priv_turn core_id, Ob~0);
+       toIMem.(MemReq.reset)();
+       toDMem.(MemReq.reset)();
+       write0(purge core_id, enum purge_state { Purged })
+    }}.
+
+  Definition tc_doMemReq0:= tc_rule R Sigma (do_mem_req CoreId0).
+  Definition tc_doMemReq1 := tc_rule R Sigma (do_mem_req CoreId1).
+  Definition tc_doMemResp0:= tc_rule R Sigma (do_mem_resp CoreId0).
+  Definition tc_doMemResp1 := tc_rule R Sigma (do_mem_resp CoreId1).
+  Definition tc_doPurge0:= tc_rule R Sigma (do_purge CoreId0).
+  Definition tc_doPurge1 := tc_rule R Sigma (do_purge CoreId1).
+  Definition tc_external_mem := tc_rule R Sigma (do_external_mem).
+  Definition tc_tick := tc_rule R Sigma do_tick_turn.
+  Definition tc_init0 := tc_rule R Sigma (do_init CoreId0).
+  Definition tc_init1 := tc_rule R Sigma (do_init CoreId1).
+
+  Definition rules (rl: mem_rules_t) : rule R Sigma :=
+    match rl with
+    | Rl_doMemReq CoreId0 => tc_doMemReq0
+    | Rl_doMemReq CoreId1=> tc_doMemReq1
+    | Rl_doMemResp CoreId0 => tc_doMemResp0
+    | Rl_doMemResp CoreId1  => tc_doMemResp1
+    | Rl_doPurge CoreId0 => tc_doPurge0
+    | Rl_doPurge CoreId1 => tc_doPurge1
+    | Rl_doExternalMem => tc_external_mem
+    | Rl_tick => tc_tick
+    | Rl_doInit CoreId0 => tc_init0
+    | Rl_doInit CoreId1 => tc_init1
+    end.
+
+  Instance Show_reg_t : Show reg_t := _.
+
+  Definition schedule : @Syntax.scheduler Frontend.pos_t mem_rules_t :=
+      Rl_doMemReq CoreId0 |> Rl_doMemReq CoreId1
+        |> Rl_doPurge CoreId0 |> Rl_doPurge CoreId1 |> Rl_doExternalMem
+                   |> Rl_doMemResp CoreId0 |> Rl_doMemResp CoreId1 |> Rl_doInit CoreId0 |> Rl_doInit CoreId1 |> Rl_tick |> done.
+
+
+
+
+  Definition metadataReq: UInternalFunction reg_t ext_fn_t :=
+    {{ fun metadataReq (req: (struct_t metadata_input)) : bits_t 0 =>
+         write0(reg_metadata_req, { valid (struct_t metadata_input) }(req) )
+    }}.
+
+  (* Four reg_metadata_req *)
+
+  Definition do_external_metadata: uaction reg_t ext_fn_t :=
+    {{
+        let req := read1(reg_metadata_req) in
+        let enqueue := get(req, valid) in
+        let memory_request := (if enqueue then get(req, req)
+                               else `UConst (tau := struct_t metadata_input) (value_of_bits Bits.zero)`) in
+        let response := extcall ext_metadata (struct metadata_input {get_ready := Ob~1;
+                                                                     put_valid := enqueue;
+                                                                     put_request := memory_request }) in
+        (if enqueue then
+           write1(reg_metadata_req, subst (req,valid,Ob~0))
+         else pass);
+        let is_response := get(response, get_valid) in
+        let response := get(response, get_response) in
+        write0(reg_metadata_resp, struct (maybe (struct_t metadata_output))
+                                         { valid := is_response;
+                                           data := response
+                                         })
+    }}.
+        (if enqueue then
+           write1(SHReq, subst (req,valid,Ob~0))
+         else pass);
+        let is_response := get(response, get_valid) in
+        let response := get(response, get_response) in
+        write0(SHResp, struct shresp { resp := response;
+                                       sourceType := get(req, sourceType);
+                                       sourceCore := get(req, sourceCore);
+                                       valid := is_response })
+
+        let
+
+
+  Definition do_external_mem : uaction reg_t ext_fn_t :=
+    {{
+        let req := read1(SHReq) in
+        let enqueue := get(req, valid) in
+        let memory_request := (if enqueue then get(req, req)
+                               else `UConst (tau := struct_t mem_req) (value_of_bits Bits.zero)`) in
+        let response := extcall ext_mainmem (struct mem_input {get_ready := Ob~1;
+                                                               put_valid := enqueue;
+                                                               put_request := memory_request }) in
+        (if enqueue then
+           write1(SHReq, subst (req,valid,Ob~0))
+         else pass);
+        let is_response := get(response, get_valid) in
+        let response := get(response, get_response) in
+        write0(SHResp, struct shresp { resp := response;
+                                       sourceType := get(req, sourceType);
+                                       sourceCore := get(req, sourceCore);
+                                       valid := is_response })
+    }}.
+
+  Definition do_mem_req (core_id: ind_core_id): uaction reg_t ext_fn_t :=
+    let fromIMem := fromIMem core_id in
+    let toIMem := toIMem core_id in
+    let fromDMem := fromDMem core_id in
+    let toDMem := toDMem core_id in
+    {{ guard(read0(purge core_id) == enum purge_state { Ready } );
+       guard(read0(turn) == #(mem_write_turn core_id));
+       (if (read0(priv_turn core_id)) then
+         if ( fromIMem.(MemRespBypass.can_enq)() && toIMem.(MemReq.can_deq)())  then
+           (let req := toIMem.(MemReq.deq)() in
+            write0(SHReq, struct shreq { req := req;
+                                         sourceType := Ob~1;
+                                         sourceCore := (#(core_id_to_bits core_id));
+                                         valid := Ob~1
+                                        })
+           )
+         else
+           pass
+       else (* (read0(priv_turn core_id) == Ob~1 *)
+         if ( fromDMem.(MemRespBypass.can_enq)() && toDMem.(MemReq.can_deq)())  then
+           (let req := toDMem.(MemReq.deq)() in
+            write0(SHReq, struct shreq { req := req;
+                                         sourceType := Ob~0;
+                                         sourceCore := (#(core_id_to_bits core_id));
+                                         valid := Ob~1
+                                        })
+           )
+         else pass);
+       write0((priv_turn core_id), read0(priv_turn core_id) + Ob~1)
+    }}.
+
+
+End Memory.
+*)
