examples/rv_isolation/RegFile.v
@@ -1,0 +1,62 @@
+(*! Implementation of a Register File *)
+Require Import Koika.Frontend.
+
+Module Type RfPow2_sig.
+  Parameter idx_sz: nat.
+  Parameter T: type.
+  Parameter init: T.
+  Parameter read_style : @switch_style var_t.
+  Parameter write_style : @switch_style var_t.
+  Parameter rf_struct_name : string.
+End RfPow2_sig.
+
+Module RfPow2 (s: RfPow2_sig).
+  Definition sz := pow2 s.idx_sz.
+  Inductive reg_t := rData (n: Vect.index sz).
+
+  Definition R r :=
+    match r with
+    | rData _ => s.T
+    end.
+
+  Definition r idx : R idx :=
+    match idx with
+    | rData _ => s.init
+    end.
+
+  Definition name_reg r :=
+    match r with
+    | rData n => String.append "rData_" (show n)
+    end.
+
+  Definition rf_write_t:=
+    {| struct_name := s.rf_struct_name;
+       struct_fields := [("arg_idx", bits_t s.idx_sz);
+                         ("arg_val", s.T)
+                        ]
+    |}.
+
+  Definition read_0 : UInternalFunction reg_t empty_ext_fn_t :=
+    {{ fun read_0 (idx : bits_t s.idx_sz) : s.T =>
+         `UCompleteSwitch s.read_style s.idx_sz "idx"
+              (fun idx => {{ read0(rData idx) }})` }}.
+
+  Definition write_0 : UInternalFunction reg_t empty_ext_fn_t :=
+    {{ fun write_0 (arg: struct_t rf_write_t) : unit_t =>
+         let idx := get(arg,arg_idx) in
+         let val := get(arg,arg_val) in
+         `UCompleteSwitch s.write_style s.idx_sz "idx"
+              (fun idx => {{ write0(rData idx, val) }})` }}.
+
+  Definition read_1 : UInternalFunction reg_t empty_ext_fn_t :=
+    {{ fun read_1 (idx : bits_t s.idx_sz) : s.T =>
+         `UCompleteSwitch s.read_style s.idx_sz "idx"
+              (fun idx => {{ read1(rData idx) }})` }}.
+
+  Definition write_1 : UInternalFunction reg_t empty_ext_fn_t :=
+    {{ fun write_1 (arg: struct_t rf_write_t) : unit_t =>
+         let idx := get(arg,arg_idx) in
+         let val := get(arg,arg_val) in
+         `UCompleteSwitch s.write_style s.idx_sz "idx"
+              (fun idx => {{ write1(rData idx, val) }})` }}.
+End RfPow2.
