examples/rv_isolation/rv32i.v
@@ -1,0 +1,5 @@
+(*! Pipelined instantiation of an RV32I core !*)
+Require Import rv_isolation.RVCore rv_isolation.rv32.
+Module RV32IPackage := Package.
+Definition prog := Interop.Backends.register RV32IPackage.package.
+Extraction "rv32i.ml" prog.
