examples/rv_cache_isolation/rv32i_extr.v
@@ -1,0 +1,2 @@
+Require Coq.extraction.Extraction rv_cache_isolation.rv32i.
+Extraction "rv32i.ml" rv32i.prog.
