examples/rv_isolation/etc/sv/top.v
@@ -1,0 +1,61 @@
+// -*- verilog -*-
+/*! Verilog wrapper for the Kôika core (for use in simulation) !*/
+// This toplevel is mostly for simulation, since it assumes the UART module
+// is always ready to transmit.
+module top(input CLK, input RST_N, output uart_wr_valid, output[7:0] uart_wr_data, output LED);
+   wire[69:0] mainmem_out;
+   wire[69:0] mainmem_arg;
+
+   wire uart_wr_ready = 1'b1;
+
+   wire uart_rd_valid = 1'b0;
+   wire[7:0] uart_rd_data = 8'b0;
+   wire uart_rd_ready;
+
+   wire led_wr_valid;
+   wire led_wr_data;
+
+   reg led = 1'b0;
+   assign LED = led;
+
+   rv32 core(.CLK(CLK), .RST_N(RST_N),
+
+             .ext_mainmem_arg(mainmem_arg),
+             .ext_mainmem_out(mainmem_out),
+
+             .ext_uart_write_arg({uart_wr_valid, uart_wr_data}),
+             .ext_uart_write_out(uart_wr_ready),
+
+             .ext_uart_read_arg(uart_rd_ready),
+             .ext_uart_read_out({uart_rd_valid, uart_rd_data}),
+
+             .ext_led_arg({led_wr_valid, led_wr_data}),
+             .ext_led_out(led));
+
+   ext_mem mainmem(.CLK(CLK), .RST_N(RST_N), .arg(mainmem_arg), .out(mainmem_out));
+
+   always @(posedge CLK)
+     if (led_wr_valid)
+       led <= led_wr_data;
+
+`ifndef STDERR
+ `define STDERR 32'h80000002
+`endif
+
+`ifdef SIMULATION
+   always @(posedge CLK) begin
+      if (led_wr_valid) begin
+         if (led_wr_data)
+           $fwrite(`STDERR, "☀");
+         else
+           $fwrite(`STDERR, "🌣");
+      end
+      if (uart_wr_ready && uart_wr_valid)
+        $fwrite(`STDERR, "%c", uart_wr_data);
+   end
+`endif
+endmodule
+
+// Local Variables:
+// flycheck-verilator-include-path: ("../../_objects/rv32i.v/")
+// End:
