examples/rv_isolation/sloc.sh
@@ -1,0 +1,13 @@
+#! /bin/sh
+
+echo "CLOC cuttlesim"
+cloc _objects/rv32i.v/rv32.hpp
+
+echo "CLOC verilator"
+cloc _objects/rv32i.v/rv32.v
+
+echo "CLOC impl"
+IMPL_FILES=("Common.v" "External.v" "Machine.v" "Memory.v" "Multiplier.v" "RegFile.v" "rv32i.v" "RVCore.v" "RVEncoding.v" "Scoreboard.v" "SecurityMonitor.v")
+cloc "${IMPL_FILES[@]}"
+
+
